The hold functions/relations should yield constants.

SynchronousNat.v
@@ -13,7 +13,7 @@ Definition cstream := nat -> bool.
 
 (* With auxiliary hold function. *)
 
-Inductive holdR (v0: const) (xs: stream) : nat -> value -> Prop :=
+Inductive holdR (v0: const) (xs: stream) : nat -> const -> Prop :=
 | holdR0:
     holdR v0 xs 0 v0
 | holdR_absent:
@@ -22,9 +22,9 @@ Inductive holdR (v0: const) (xs: stream) : nat -> value -> Prop :=
       holdR v0 xs n v ->
       holdR v0 xs (S n) v
 | holdR_present:
-    forall n,
-      xs n <> absent ->
-      holdR v0 xs (S n) (xs n).
+    forall n c,
+      xs n = present c ->
+      holdR v0 xs (S n) c.
 
 Inductive fbyR (v0: const) (xs: stream) : nat -> value -> Prop :=
 | fbyR_absent:
@@ -37,12 +37,12 @@ Inductive fbyR (v0: const) (xs: stream) : nat -> value -> Prop :=
       holdR v0 xs n v ->
       fbyR v0 xs n v.
 
-Fixpoint hold (v0: const) (xs: stream) (n: nat) : value :=
+Fixpoint hold (v0: const) (xs: stream) (n: nat) : const :=
   match n with
   | 0 => v0
   | S m => match xs m with
            | absent => hold v0 xs m
-           | hv => hv
+           | present hv => hv
            end
   end.
 
@@ -58,18 +58,21 @@ Proof.
   - cbv; auto using holdR0.
   - simpl. case_eq (xs n).
     + auto using holdR_absent.
-    + intros v xsn; rewrite <- xsn.
+    + intros v xsn.
       apply holdR_present.
-      rewrite xsn; discriminate.
+      apply xsn.
 Qed.
 
-Lemma hold_rel2: forall v0 xs n v, holdR v0 xs n v -> hold v0 xs n = v.
+Lemma hold_rel2: forall v0 xs n c, holdR v0 xs n c -> hold v0 xs n = c.
 Proof.
   induction n as [|n IH].
   - inversion 1; auto.
-  - intros v H; inversion_clear H as [|? ? xsn HR|? H1].
+  - intros v H; inversion_clear H as [|? ? xsn HR|? H1 H2].
     + simpl; rewrite xsn; apply (IH v HR).
-    + simpl. case_eq (xs n). contradiction. trivial.
+    + simpl. case_eq (xs n).
+      rewrite H2; intro H1; discriminate H1.
+      intros v1 H3; rewrite H3 in H2; injection H2.
+      trivial.
 Qed.
 
 Lemma hold_rel: forall v0 xs n v, hold v0 xs n = v <-> holdR v0 xs n v.
@@ -78,7 +81,7 @@ Proof.
   intro H; rewrite <- H; apply hold_rel1.
   apply hold_rel2.
 Qed.
-    
+
 Lemma fby_rel1: forall v0 xs n, fbyR v0 xs n (fby v0 xs n).
 Proof.
   intros v0 xs n.
@@ -97,11 +100,17 @@ Proof.
   - inversion_clear 1 as [ ? H0 | ? ? ? HR].
     + unfold fby; rewrite H0; reflexivity.
     + unfold fby; case_eq (xs 0).
-      contradiction. intros v1 xsn; apply hold_rel2; exact HR.
+      contradiction.
+      intros v2 xsn.
+      apply hold_rel2 in HR; inversion HR.
+      trivial.
   - inversion_clear 1 as [ ? H0 | ? ? ? HR].
     + unfold fby; rewrite H0; reflexivity.
     + unfold fby; case_eq (xs (S n)).
-      contradiction. intros v1 xsn; apply hold_rel2; exact HR.
+      contradiction.
+      intros v2 xsn.
+      apply hold_rel2 in HR; inversion HR.
+      trivial.
 Qed.
 
 Lemma fby_rel: forall v0 xs n v, fby v0 xs n = v <-> fbyR v0 xs n v.
